src/lib/kuiper/Kuiper.SizeT.fst
@@ -1,0 +1,64 @@
+module Kuiper.SizeT
+
+let fits_iff_u32 (x:nat)
+  : Lemma (FStar.SizeT.fits x <==> FStar.UInt.fits x 32)
+          [SMTPat (FStar.SizeT.fits x)]
+  = admit() (* assumption *)
+
+(* This is extracted primitely, it must not be marked inline. *)
+let sizet_to_u32 (x: SZ.t)
+  : Pure U32.t (requires FStar.UInt.fits (SZ.v x) 32)
+               (ensures fun r -> U32.v r == SZ.v x)
+  = U32.uint_to_t (SZ.v x)
+
+(* This is extracted primitively, it must not be marked inline. *)
+let sizet_and (x y : SZ.t) : SZ.t =
+  magic ()
+
+let sizet_and_div_pow2 (x:SZ.t) (y:SZ.t) (n:nat)
+  : Lemma (requires SZ.v y == pow2 n)
+          (ensures SZ.v (sizet_and x SZ.(y -^ 1sz)) == SZ.v x % (pow2 n))
+  = admit() (* assumption, should prove it! *)
+
+let s_divmod_inv_1 (j:szp) (i:sz)
+  : Lemma (s_undivmod j (s_divmod j i) == i)
+          [SMTPat (s_undivmod j (s_divmod j i))]
+  = ()
+
+let s_divmod_inv_2 (j:szp) (dm : sz & szlt j {SZ.fits (dm._1 * j + dm._2)})
+  : Lemma (s_divmod j (s_undivmod j dm) == dm)
+          [SMTPat (s_divmod j (s_undivmod j dm))]
+  = ()
+
+let lem_sdivup (x:sz) (y:szp{SZ.fits (x+y)})
+  : Lemma (SZ.v (sdivup x y) == divup (SZ.v x) (SZ.v y))
+          [SMTPat (sdivup x y)]
+  = ()
+
+inline_for_extraction noextract
+let spow2 (s : sz{s < 32}) : r:sz{SZ.v r == pow2 s} =
+  SZ.uint32_to_sizet (U32.shift_left 1ul (sizet_to_u32 s))
+
+inline_for_extraction noextract
+let sdiv_pow2 (i:sz{i < 32}) (tid: sz) : bool =
+  // SZ.rem tid (spow2 i) = 0sz
+  sizet_and tid SZ.(spow2 i -^ 1sz) = 0sz
+
+let sdiv_pow2_ok (i:sz{i < 32}) (tid:sz) :
+  Lemma (sdiv_pow2 i tid == div_pow2 i tid)
+        [SMTPat (sdiv_pow2 i tid)]
+= sizet_and_div_pow2 tid (spow2 i) i;
+  calc (==) {
+    SZ.v (SZ.rem tid (spow2 i));
+    == {}
+    SZ.v tid - ((SZ.v tid / SZ.v (spow2 i)) * SZ.v (spow2 i));
+    == { FStar.Math.Lemmas.euclidean_division_definition (SZ.v tid) (SZ.v (spow2 i)) }
+    SZ.v tid % SZ.v (spow2 i);
+    == {}
+    SZ.v tid % pow2 (SZ.v i);
+}
+
+noextract inline_for_extraction
+let smin (a b : sz): sz =
+  let open FStar.SizeT in
+  if a <^ b then a else b
